\section{Beta-Bernoulli model}
$\mathcal D = \{x_n : x_n \sim \Ber(\theta)\}, \theta \sim \Beta(\alpha, \beta)$.

\paragraph{Likelihood.}
\begin{align*}
    p(\mathcal D \mid \theta)   &= \theta^{N_1} (1 - \theta)^{N_0}
\end{align*}
where $N_1 = \sum_n \I(x_n = 1)$ and $N_0 = \sum_n \I(x_n = 0)$.

\paragraph{Posterior.}
\begin{align*}
    p(\theta \mid \mathcal D)   &\propto p(\mathcal D \mid \theta) p(\theta) \\
                                &\propto \theta^{N_1} (1 - \theta)^{N_0} \theta^{\alpha - 1} (1 - \theta)^{\beta - 1} \\
                                &= \theta^{\alpha + N_1 - 1} (1 - \theta)^{\beta + N_0 - 1} \\
                                &\propto \Beta(\theta \mid \alpha + N_1, \beta + N_0)
\end{align*}

\paragraph{Posterior predictive.}
\begin{align*}
    p(\tilde x = 1 \mid \mathcal D) &= \int_{\theta} p(\tilde x, \theta \mid \mathcal D) \,\mathrm d\theta \\
                                    &= \int_{\theta} p(\tilde x \mid \theta, \mathcal D) p(\theta \mid \mathcal D) \,\mathrm d\theta \\
                                    &= \int_{\theta} p(\tilde x \mid \theta) p(\theta \mid \mathcal D) \,\mathrm d\theta \\
                                    &= \int_{\theta} \theta \Beta(\theta, \alpha', \beta') \,\mathrm d \theta \\
                                    &= \E_{\theta \sim \Beta(\alpha', \beta')}[\theta] \\
                                    &= \frac{\alpha'}{\alpha' + \beta'} \\
    \implies \tilde x               &\sim \Ber\left(\frac{\alpha'}{\alpha' + \beta'}\right)
\end{align*}