\section{Poisson-Gamma model}
$\mathcal D = \{x_n : x_n \sim \Poi(\lambda)$, $\lambda \sim \Gammadist(\alpha, \beta)$.

\paragraph{Likelihood.}
    \begin{align*}
        p(\mathcal D \mid \lambda) &= \prod_n \Poi(x_n \mid \lambda)
    \end{align*}

\paragraph{Posterior.}
    \begin{align*}
        p(\lambda \mid \mathcal D)  &\propto p(\mathcal D \mid \lambda) p(\lambda) \\
                                    &= \left(\prod_n \Poi(x_n \mid \lambda) \right) \Gammadist(\lambda \mid \alpha, \beta) \\
                                    &\propto \left[\prod_n \frac{\lambda^{x_n}}{x_n!} \exp(-\lambda)\right] \left[\lambda^{\alpha - 1} \exp(-\lambda\beta)\right] \\
                                    &\propto \lambda^{\alpha + \sum_n x_n - 1} \exp(-\lambda(\beta + N)) \\
                                    &\propto \Gammadist\left(\lambda \mid \alpha + \sum_n x_n, \beta + N\right)
    \end{align*}

\paragraph{Posterior predictive.}
    \begin{align*}
        p(\tilde x \mid \mathcal D) &= \int_{\lambda} p(\tilde x, \lambda \mid \mathcal D) \,\mathrm d\lambda \\
                                    &= \int_{\lambda} p(\tilde x \mid \lambda, \mathcal D) p(\lambda \mid \mathcal D) \,\mathrm d\lambda \\
                                    &= \int_{\lambda} p(\tilde x \mid \lambda) p(\lambda \mid \mathcal D) \,\mathrm d\lambda \\
                                    &= \int_{\lambda} \Poi(\tilde x \mid \lambda) \Gammadist(\lambda \mid \alpha', \beta') \,\mathrm d\lambda \\
                                    &= \int_{\lambda} \frac{\lambda^{\tilde x}}{\tilde x!} \exp(-\lambda) \frac{1}{G(\alpha', \beta')} \lambda^{\alpha' - 1} \exp(-\beta' \lambda) \,\mathrm d\lambda \\
                                    &= \frac{1}{\tilde x! G(\alpha', \beta')} \int_{\lambda} \lambda^{x + \alpha' - 1} \exp(-\lambda (\beta' + 1)) \,\mathrm d\lambda \\
                                    &= \frac{G(\alpha' + x, \beta + 1)}{\tilde x! G(\alpha', \beta')} \\
                                    &= \frac{\Gamma(\alpha' + \tilde x)}{\tilde x! \Gamma(\alpha')} \cdot \frac{\beta'^{\alpha'}}{(\beta' + 1)^{\alpha' + \tilde x}} \\
                                    &= \frac{\Gamma(\alpha' + \tilde x)}{\tilde x! \Gamma(\alpha')} \left(1 - \frac{1}{1 + \beta'}\right)^{\alpha'} \left(\frac{1}{1 + \beta'}\right)^{\tilde x} \\
                                    &= \NB\left(\tilde x \mid \alpha', \frac{1}{1 + \beta'}\right)
    \end{align*}
where $G(\alpha, \beta)$ is the normalisation constant for a Gamma distribution, $\Gammadist(\alpha, \beta)$, which is $\int_x x^{\alpha - 1} \exp(-\beta x) \,\mathrm dx$ or $\frac{\Gamma(\alpha)}{\beta^\alpha}$.